Meta.Test.Class.Equiv: more

coq/ZF/Meta/Test/Class/Equiv.v
@@ -83,6 +83,94 @@ Definition EquivCompatR : Term :=
             (Ident "equiv" [Var 2; Var 1])
             (Ident "equiv" [Var 2; Var 0]))))).
 
+(* Proposition Sym : forall P Q, equiv P Q -> equiv Q P.                        *)
+Definition Sym : Term :=
+  All VarTyClass
+    (All VarTyClass
+      (Imp
+        (Ident "equiv" [Var 1; Var 0])
+        (Ident "equiv" [Var 0; Var 1]))).
+
+(* Proposition Tran : forall P Q R,                                             *)
+(* equiv P Q -> equiv Q R -> equiv P R.                                         *)
+Definition Tran : Term :=
+  All VarTyClass
+    (All VarTyClass
+      (All VarTyClass
+        (Imp
+          (Ident "equiv" [Var 2; Var 1])
+          (Imp
+            (Ident "equiv" [Var 1; Var 0])
+            (Ident "equiv" [Var 2; Var 0]))))).
+
+(* Proposition NotSym : forall P Q, ~ equiv P Q -> ~ equiv Q P.                 *)
+Definition NotSym : Term :=
+  All VarTyClass
+    (All VarTyClass
+      (Imp
+        (Not (Ident "equiv" [Var 1; Var 0]))
+        (Not (Ident "equiv" [Var 0; Var 1])))).
+
+(* Proposition EqualToClass : forall a b,                                       *)
+(* a = b <-> equiv (toClass a) (toClass b).                                     *)
+Definition EqualToClass : Term :=
+  All VarTySet
+    (All VarTySet
+      (Iff
+        (Equal (Var 1) (Var 0))
+        (Ident "equiv"
+          [Ident "toClass" [Var 1]; Ident "toClass" [Var 0]]))).
+
+(* Proposition NotEqualToClass : forall a b,                                    *)
+(* a <> b <-> ~ equiv (toClass a) (toClass b).                                  *)
+Definition NotEqualToClass : Term :=
+  All VarTySet
+    (All VarTySet
+      (Iff
+        (NotEq (Var 1) (Var 0))
+        (Not
+          (Ident "equiv"
+            [Ident "toClass" [Var 1]; Ident "toClass" [Var 0]])))).
+
+(* Proposition NotCompat : forall P Q R S,                                      *)
+(* equiv P Q -> equiv R S -> ~ equiv P R -> ~ equiv Q S.                        *)
+Definition NotCompat : Term :=
+  All VarTyClass
+    (All VarTyClass
+      (All VarTyClass
+        (All VarTyClass
+          (Imp
+            (Ident "equiv" [Var 3; Var 2])
+            (Imp
+              (Ident "equiv" [Var 1; Var 0])
+              (Imp
+                (Not (Ident "equiv" [Var 3; Var 1]))
+                (Not (Ident "equiv" [Var 2; Var 0])))))))).
+
+(* Proposition NotCompatL : forall P Q R,                                       *)
+(* equiv P Q -> ~ equiv P R -> ~ equiv Q R.                                     *)
+Definition NotCompatL : Term :=
+  All VarTyClass
+    (All VarTyClass
+      (All VarTyClass
+        (Imp
+          (Ident "equiv" [Var 2; Var 1])
+          (Imp
+            (Not (Ident "equiv" [Var 2; Var 0]))
+            (Not (Ident "equiv" [Var 1; Var 0])))))).
+
+(* Proposition NotCompatR : forall P Q R,                                       *)
+(* equiv P Q -> ~ equiv R P -> ~ equiv R Q.                                     *)
+Definition NotCompatR : Term :=
+  All VarTyClass
+    (All VarTyClass
+      (All VarTyClass
+        (Imp
+          (Ident "equiv" [Var 2; Var 1])
+          (Imp
+            (Not (Ident "equiv" [Var 0; Var 2]))
+            (Not (Ident "equiv" [Var 0; Var 1])))))).
+
 (* Declaration typing.                                                          *)
 
 (* The declaration body for toClass maps a set to its membership class.         *)
@@ -118,6 +206,19 @@ Proof.
   - apply HasTysNil.
 Qed.
 
+(* The identifier toClass sends any set variable to a class.                    *)
+Proposition toClassVarHasTy : forall (G:Ctx) (n:nat),
+  typeOf G n = Some TySet ->
+  HasTyIn env G (Ident "toClass" [Var n]) TyClass.
+Proof.
+  (* Proof by Hermes + gpt 5.5                                                  *)
+  intros G n H1.
+  apply HasTyIdent with (argTys := [TySet]). 1: reflexivity.
+  apply HasTysCons.
+  - apply HasTyVar. assumption.
+  - apply HasTysNil.
+Qed.
+
 (* The identifier equiv sends two class arguments to a proposition.             *)
 Proposition equivHasTy :
   HasTyIn env [TyClass; TyClass]
@@ -146,6 +247,18 @@ Proof.
   - apply HasTysCons.
     + apply HasTyVar. assumption.
     + apply HasTysNil.
+Qed.
+
+(* Negated equivalence of two class variables is well sorted.                   *)
+Proposition notEquivVarsHasTy : forall (G:Ctx) (m n:nat),
+  typeOf G m = Some TyClass ->
+  typeOf G n = Some TyClass ->
+  HasTyIn env G (Not (Ident "equiv" [Var m; Var n])) TyProp.
+Proof.
+  (* Proof by Hermes + gpt 5.5                                                  *)
+  intros G m n H1 H2.
+  apply HasTyNot.
+  apply equivVarsHasTy; assumption.
 Qed.
 
 (* Proposition typing.                                                          *)
@@ -192,4 +305,88 @@ Proof.
   apply HasTyAll, HasTyAll, HasTyAll, HasTyImp.
   - apply equivVarsHasTy; reflexivity.
   - apply HasTyImp; apply equivVarsHasTy; reflexivity.
+Qed.
+
+(* Symmetry of equivalence is a well-sorted proposition.                        *)
+Proposition SymHasTy : HasTyIn env Ctx.empty Sym TyProp.
+Proof.
+  (* Proof by Hermes + gpt 5.5                                                  *)
+  apply HasTyAll, HasTyAll, HasTyImp; apply equivVarsHasTy; reflexivity.
+Qed.
+
+(* Transitivity of equivalence is a well-sorted proposition.                    *)
+Proposition TranHasTy : HasTyIn env Ctx.empty Tran TyProp.
+Proof.
+  (* Proof by Hermes + gpt 5.5                                                  *)
+  apply HasTyAll, HasTyAll, HasTyAll, HasTyImp.
+  - apply equivVarsHasTy; reflexivity.
+  - apply HasTyImp; apply equivVarsHasTy; reflexivity.
+Qed.
+
+(* Symmetry of non-equivalence is a well-sorted proposition.                    *)
+Proposition NotSymHasTy : HasTyIn env Ctx.empty NotSym TyProp.
+Proof.
+  (* Proof by Hermes + gpt 5.5                                                  *)
+  apply HasTyAll, HasTyAll, HasTyImp; apply notEquivVarsHasTy; reflexivity.
+Qed.
+
+(* Equality of sets and equivalence of their classes is well sorted.            *)
+Proposition EqualToClassHasTy : HasTyIn env Ctx.empty EqualToClass TyProp.
+Proof.
+  (* Proof by Hermes + gpt 5.5                                                  *)
+  apply HasTyAll, HasTyAll, HasTyIff.
+  - apply HasTyEqual; apply (HasTyVar _ _ _ TySet); reflexivity.
+  - apply HasTyIdent with (argTys := [TyClass; TyClass]). 1: reflexivity.
+    apply HasTysCons.
+    + apply toClassVarHasTy. reflexivity.
+    + apply HasTysCons.
+      * apply toClassVarHasTy. reflexivity.
+      * apply HasTysNil.
+Qed.
+
+(* Inequality of sets and non-equivalence of their classes is well sorted.      *)
+Proposition NotEqualToClassHasTy :
+  HasTyIn env Ctx.empty NotEqualToClass TyProp.
+Proof.
+  (* Proof by Hermes + gpt 5.5                                                  *)
+  apply HasTyAll, HasTyAll, HasTyIff.
+  - apply HasTyNotEq; apply (HasTyVar _ _ _ TySet); reflexivity.
+  - apply HasTyNot.
+    apply HasTyIdent with (argTys := [TyClass; TyClass]). 1: reflexivity.
+    apply HasTysCons.
+    + apply toClassVarHasTy. reflexivity.
+    + apply HasTysCons.
+      * apply toClassVarHasTy. reflexivity.
+      * apply HasTysNil.
+Qed.
+
+(* Non-equivalence is compatible with equivalence.                              *)
+Proposition NotCompatHasTy : HasTyIn env Ctx.empty NotCompat TyProp.
+Proof.
+  (* Proof by Hermes + gpt 5.5                                                  *)
+  apply HasTyAll, HasTyAll, HasTyAll, HasTyAll, HasTyImp.
+  - apply equivVarsHasTy; reflexivity.
+  - apply HasTyImp.
+    + apply equivVarsHasTy; reflexivity.
+    + apply HasTyImp.
+      * apply notEquivVarsHasTy; reflexivity.
+      * apply notEquivVarsHasTy; reflexivity.
+Qed.
+
+(* Non-equivalence is left-compatible with equivalence.                         *)
+Proposition NotCompatLHasTy : HasTyIn env Ctx.empty NotCompatL TyProp.
+Proof.
+  (* Proof by Hermes + gpt 5.5                                                  *)
+  apply HasTyAll, HasTyAll, HasTyAll, HasTyImp.
+  - apply equivVarsHasTy; reflexivity.
+  - apply HasTyImp; apply notEquivVarsHasTy; reflexivity.
+Qed.
+
+(* Non-equivalence is right-compatible with equivalence.                        *)
+Proposition NotCompatRHasTy : HasTyIn env Ctx.empty NotCompatR TyProp.
+Proof.
+  (* Proof by Hermes + gpt 5.5                                                  *)
+  apply HasTyAll, HasTyAll, HasTyAll, HasTyImp.
+  - apply equivVarsHasTy; reflexivity.
+  - apply HasTyImp; apply notEquivVarsHasTy; reflexivity.
 Qed.
